proper proof building

Reflection.v
@@ -8,7 +8,6 @@ Require Import Tarski.
 Require Import VectorTech.
 Require Import Lia.
 
-
 (* I follow the treatment of Peter Smith in "Introduction to Gödel's Theorems"
  (page 37) *)
 
@@ -61,9 +60,6 @@ Fixpoint num n :=
   | S x => σ (num x)
   end.
 
-                      
-
-
 (* formulate axioms of PA (see page 92) *)
 
 Definition ax_zero_succ := ∀    zero == σ var 0 --> fal.
@@ -77,8 +73,8 @@ Definition ax_mult_rec :=  ∀ ∀  σ $1 ⊗ $0 == $0 ⊕ $1 ⊗ $0.
 Definition PA_induction (phi : form) :=
   phi[zero..] --> (∀ phi --> phi[σ $0 .: S >> var]) --> ∀ phi.
 Definition phi := $0 == $1.
-Compute (phi[zero..]).
-Compute (phi[zero .: S >> var]).
+(*Compute (phi[zero..]).
+  Compute (phi[zero .: S >> var]).*)
 
 (* substitutes t for the variable $0 and leaves all other variables unchanged *)
 Definition var0_subst (t : term) : nat -> term :=
@@ -95,23 +91,19 @@ Qed.
 
 
 
-                                              
-
 (*** Working in models of PA ***)
-                                              
-Section Models.                                              
+
+Section Models.
 
   Variable D : Type.
   Context {I : interp D}.
-
-  Definition Equality := forall v, @i_P _ _ D I Eq v <-> Vector.hd v = Vector.hd (Vector.tl v). 
-  Hypothesis equality : forall v, @i_P _ _ D I Eq v <-> Vector.hd v = Vector.hd (Vector.tl v).
 
   Notation iO := (i_f (f:=Zero) (Vector.nil D)).
   Notation "'iσ' d" := (i_f (f:=Succ) (Vector.cons d (Vector.nil D))) (at level 37).
   Notation "x 'i⊕' y" := (i_f (f:=Plus) (Vector.cons x (Vector.cons y (Vector.nil D)))) (at level 39).
   Notation "x 'i⊗' y" := (i_f (f:=Mult) (Vector.cons x (Vector.cons y (Vector.nil D)))) (at level 38).
   Notation "x 'i=' y" := (i_P (P:=Eq)   (Vector.cons x (Vector.cons y (Vector.nil D)))) (at level 40).
+  Hypothesis equality : forall a b, a i= b <-> a = b.
   Definition iμ k := iter (fun x => iσ x) k iO.
   Fixpoint naryProp (n:nat) : Type := match n with 0 => Prop | S nn => D -> naryProp nn end.
   Fixpoint representsP {n:nat} phi rho : (forall (P:naryProp n), Prop) := match n return (forall (P:naryProp n), Prop) with
@@ -120,6 +112,79 @@ Section Models.
   Definition representableP (n:nat) (P : naryProp n) := exists phi rho, representsP phi rho P.
   Definition representsF (d:D) trm rho := eval rho trm = d.
   Definition representableF (d:D) := exists trm rho, representsF d trm rho.
+
+Definition mergeAnd (rho:nat -> D) (P Q : naryProp 0) : {phi:form & representsP phi rho P} -> {phi:form & representsP phi rho Q} -> {phi:form & @representsP 0 phi rho (P /\ Q)}.
+Proof.
+intros [phiP HP] [phiQ HQ].
+pose (phiP∧phiQ). exists f. destruct HP as [pPl pPr]. destruct HQ as [pQl pQr]. unfold f. split.
+* intros [pP pQ]. split. now apply pPl. now apply pQl.
+* intros [pP pQ]. split. now apply pPr. now apply pQr.
+Defined.
+
+Definition mergeFalse (rho:nat -> D) : {phi:form & @representsP 0 phi rho False}.
+Proof. exists fal. easy. Defined.
+
+Definition mergeOr (rho:nat -> D) (P Q : naryProp 0) : {phi:form & representsP phi rho P} -> {phi:form & representsP phi rho Q} -> {phi:form & @representsP 0 phi rho (P \/ Q)}.
+Proof.
+intros [phiP HP] [phiQ HQ].
+pose (phiP∨phiQ). exists f. destruct HP as [pPl pPr]. destruct HQ as [pQl pQr]. unfold f. split.
+* intros [pP|pQ]. left; now apply pPl. right; now apply pQl.
+* intros [pP|pQ]. left; now apply pPr. right; now apply pQr.
+Defined.
+
+Definition mergeImpl (rho:nat -> D) (P Q : naryProp 0) : {phi:form & representsP phi rho P} -> {phi:form & representsP phi rho Q} -> {phi:form & @representsP 0 phi rho (P -> Q)}.
+Proof.
+intros [phiP HP] [phiQ HQ].
+pose (phiP-->phiQ). exists f. destruct HP as [pPl pPr]. destruct HQ as [pQl pQr]. unfold f. split.
+* intros PQ pP. apply pQl, PQ, pPr, pP.
+* cbn. intros pPQ pP. apply pQr, pPQ, pPl, pP.
+Defined.
+
+Definition mergeExists (rho:nat -> D) (P:naryProp 1) : {phi:form & representsP phi rho P} -> {phi:form & @representsP 0 phi rho (exists q:D, P q)}.
+Proof.
+intros [phi pR].
+pose (∃ phi). exists f. split.
+* intros [q Pq]. exists q. destruct (pR q) as [pRl pRr]. now apply pRl.
+* intros [q Pq]. exists q. destruct (pR q) as [pRl pRr]. now apply pRr.
+Defined.
+(*
+Definition mergeForall (rho:nat -> D) (P:naryProp 1) : {phi:form & representsP phi rho P} -> {phi:form & @representsP 0 phi rho (forall q:D, P q)}.
+Proof.
+intros [phi pR].
+pose (∀ phi). exists f. split.
+* intros H q. destruct (pR q) as [pRl pRr]. now apply pRl, H.
+* intros H q. destruct (pR q) as [pRl pRr]. now apply pRr, H.
+Defined.*)
+
+Definition mergeZero (rho:nat -> D) :{phi:term & representsF (iO) phi rho}.
+Proof.
+exists zero. easy.
+Defined.
+
+Definition mergeSucc (rho:nat -> D) (d:D) : {phi:term & representsF d phi rho} -> {phi:term & representsF (iσ d) phi rho}.
+Proof. intros [t pt].
+pose (σ t). exists t0. unfold t0. unfold representsF. cbn. now rewrite pt.
+Defined.
+
+Definition mergeAdd (rho:nat -> D) (d1 d2:D) : {phi:term & representsF d1 phi rho} -> {phi:term & representsF d2 phi rho} -> {phi:term & representsF (d1 i⊕ d2) phi rho}.
+Proof. intros [t1 pt1] [t2 pt2].
+pose (t1 ⊕ t2). exists t. unfold t. unfold representsF. cbn. now rewrite pt1, pt2.
+Defined.
+
+Definition mergeMul (rho:nat -> D) (d1 d2:D) : {phi:term & representsF d1 phi rho} -> {phi:term & representsF d2 phi rho} -> {phi:term & representsF (d1 i⊗ d2) phi rho}.
+Proof. intros [t1 pt1] [t2 pt2].
+pose (t1 ⊗ t2). exists t. unfold t. unfold representsF. cbn. now rewrite pt1, pt2.
+Defined.
+
+Definition mergeEq (rho:nat -> D) (d1 d2 : D) : {phi:term & representsF d1 phi rho} -> {phi:term & representsF d2 phi rho} -> {phi:form & @representsP 0 phi rho (d1 i= d2)}.
+Proof. intros [t1 pt1] [t2 pt2].
+pose (t1 == t2). exists f. cbn. now rewrite pt1, pt2.
+Defined.
+
+Definition mergeEqProp (rho:nat -> D) (d1 d2 : D) : {phi:term & representsF d1 phi rho} -> {phi:term & representsF d2 phi rho} -> {phi:form & @representsP 0 phi rho (d1 = d2)}.
+Proof. intros [t1 pt1] [t2 pt2].
+pose (t1 == t2). exists f. cbn. now rewrite pt1, pt2.
+Defined.
 
 Notation vectorCons x T n xr := 
 (tApp
@@ -134,10 +199,8 @@ Notation vectorNil T :=
     {|
     inductive_mind := (MPfile (["VectorDef"; "Vectors"; "Coq"]), "t");
     inductive_ind := 0 |} 0 nil) ([T])).
-Notation termConstructorBase l := 
-(tApp (tConst (MPfile (["Tarski"; "Arith"]), "i_f") nil) l).
-Notation propConstructorBase l := 
-(tApp (tConst (MPfile (["Tarski"; "Arith"]), "i_P") nil) l).
+Notation termConstructorBase := (tConst (MPfile (["Tarski"; "Arith"]), "i_f") nil).
+Notation propConstructorBase := (tConst (MPfile (["Tarski"; "Arith"]), "i_P") nil).
 Definition termPropRepStart := 
    ([tConst (MPfile (["Reflection"; "Arith"]), "PA_funcs_signature") nil;
    tConst (MPfile (["Reflection"; "Arith"]), "PA_preds_signature") nil; tVar "D"; 
@@ -155,103 +218,259 @@ Fixpoint popListStart (l : list Ast.term) (ls : list Ast.term) : option (list As
 | (lx::lxr, lsx::lsxr) => if Checker.eq_term init_graph lx lsx then popListStart lxr lsxr else None
 | _ => None end.
 
-Definition failEnv (n:nat) : (TemplateMonad term):= tmFail ("Unbound " ++ string_of_nat n).
-Definition relLift (k : TemplateMonad term) : (TemplateMonad term) := kv <- k ;; match kv with var n => ret (var (S n)) | v => ret v end.
-Definition appendZero (k:TemplateMonad term) (v:nat -> TemplateMonad term) (n:nat) := match n with 0 => k | S n => v n end.
-Definition appendAndLift (k:TemplateMonad term) (v:nat -> TemplateMonad term) := appendZero k (v >> relLift).
+Definition FUEL := 100. 
 
-Definition FUEL := 100.
+Definition termReifier := list Ast.term -> Ast.term -> (Ast.term -> TemplateMonad (prod term Ast.term)) -> TemplateMonad (prod term Ast.term).
+Definition reifyZero : termReifier := fun l env fTR => match l with nil => v <- tmQuote mergeZero;;ret (pair (zero) (tApp (v) ([env]))) | _ => tmFail "Zero constructor applied to != 0 terms" end.
+Definition reifySucc : termReifier := fun l env fTR => match l with [x] => 
+                                           v <- tmQuote (mergeSucc);;
+                                           '(tx,xr) <- fTR x ;; ret (σ tx,tApp v ([env;x;xr])) | _ => tmFail "Succ constructor applied to != 1 terms" end.
+Definition reifyAdd : termReifier := fun l env fTR => match l with [x; y] =>  
+                                           v <- tmQuote (mergeAdd) ;;
+                                           '(tx,xr) <- fTR x ;; '(ty,yr) <- fTR y ;; ret (tx⊕ty,tApp v ([env;x;y;xr;yr])) | _ => tmFail "Add constructor applied to != 2 terms" end.
+Definition reifyMul : termReifier := fun l env fTR => match l with [x; y] =>  
+                                           v <- tmQuote (mergeMul) ;;
+                                           '(tx,xr) <- fTR x ;; '(ty,yr) <- fTR y ;; ret (tx⊗ty,tApp v ([env;x;y;xr;yr])) | _ => tmFail "Mul constructor applied to != 2 terms" end.
+Definition reifyTerm (n:nat) : termReifier := match n with
+0 => reifyZero | 1 => reifySucc | 2 => reifyAdd | 3 => reifyMul | _ => fun _ _ _ => tmFail ("Unknown term constructor index " ++ string_of_nat n) end.
+Definition reifyRelHelper (rho:nat -> D) (d:D) (n:nat) (H:rho n = d) : {phi:term & representsF d phi rho}.
+Proof.
+exists ($n). exact H.
+Defined.
 
-Definition termReifier (t:Type) := list Ast.term -> (Ast.term -> TemplateMonad t) -> TemplateMonad t.
-Definition reifyZero : termReifier term := fun l fTR => match l with nil => ret zero | _ => tmFail "Zero constructor applied to != 0 terms" end.
-Definition reifySucc : termReifier term := fun l fTR => match l with [x] => 
-                                           xr <- fTR x ;; ret (σ xr) | _ => tmFail "Succ constructor applied to != 1 terms" end.
-Definition reifyAdd : termReifier term := fun l fTR => match l with [x; y] =>  
-                                           xr <- fTR x ;; yr <- fTR y ;; ret (xr ⊕ yr) | _ => tmFail "Add constructor applied to != 2 terms" end.
-Definition reifyMul : termReifier term := fun l fTR => match l with [x; y] =>  
-                                           xr <- fTR x ;; yr <- fTR y ;; ret (xr ⊗ yr) | _ => tmFail "Mul constructor applied to != 2 terms" end.
-Definition reifyTerm (n:nat) : termReifier term := match n with
-0 => reifyZero | 1 => reifySucc | 2 => reifyAdd | 3 => reifyMul | _ => fun _ _ => tmFail ("Unknown term constructor index " ++ string_of_nat n) end.
 
 
 Notation termRepDet i v := (([tConstruct {| inductive_mind := (MPfile (["Reflection"; "Arith"]), "PA_funcs"); inductive_ind := 0 |}
      i nil; v])).
 Notation formRepDet i v := (([tConstruct {| inductive_mind := (MPfile (["Reflection"; "Arith"]), "PA_preds"); inductive_ind := 0 |}
      i nil; v])).
+MetaCoq Quote Definition zeroEnv := (fun k:nat => iO).
+MetaCoq Quote Definition qeq_refl := (@eq_refl).
 
-
-Fixpoint findTermRepresentation (fuel:nat) (t:Ast.term) (env:nat->TemplateMonad term) {struct fuel}: (TemplateMonad term) := 
-  let fail :=tmPrint t;;tmFail ("Cannot represent term") in match fuel with 
+Fixpoint findTermRepresentation (fuel:nat) (t:Ast.term) (termEnv:Ast.term) (env:Ast.term -> TemplateMonad nat) {struct fuel}: (TemplateMonad (prod term Ast.term)) := 
+  let fail := (v <- tmQuote reifyRelHelper;;envv <- env (t);;num <- tmQuote (envv);;ret ($envv,tApp v ([termEnv;t;num;tApp qeq_refl ([tVar "D";t])]))) in match fuel with 
     0 => tmFail "Out of fuel" 
     | S fuel => match t with
-        termConstructorBase l => match popListStart l termPropRepStart with
-          Some (termRepDet i v) => vr <- recoverVector v;;reifyTerm i vr (fun t => findTermRepresentation fuel t env)
+        tApp termConstructorBase l => match popListStart l termPropRepStart with
+          Some (termRepDet i v) => vr <- recoverVector v;;reifyTerm i vr termEnv (fun t => findTermRepresentation fuel t termEnv env)
          | _ => fail end
-      | tRel k => env k
       | _ => fail
     end 
   end.
 
-MetaCoq Run (a <- tmQuote (iO i⊕ iσ iO);;t <- findTermRepresentation FUEL a failEnv;;tmPrint t).
 
-Definition envTermReifier (t:Type) := list Ast.term -> nat -> (nat -> TemplateMonad term) -> (Ast.term -> TemplateMonad t) -> TemplateMonad t.
-Definition refiyEq : envTermReifier form := fun l fuel env fPR => match l with [x; y] =>  
-                                           xr <- findTermRepresentation fuel x env ;;
-                                           yr <- findTermRepresentation fuel y env ;; 
-                                           ret (xr == yr) | _ => tmFail "Eq constructor applied to != 2 terms" end.
-Definition reifyForm (n:nat) : envTermReifier form := match n with 0 => refiyEq | _ => fun _ _ _ _ => tmFail ("Unknown form constructor index " ++ string_of_nat n) end.
+Definition proj1 {A:Type} {B:A -> Type} : {a:A & B a} -> A := fun z => match z with existT x _ => x end.
+Definition mergeForall2 (rho:nat -> D) (Q:naryProp 0) (H:{PP : naryProp 1 & (forall x:D, PP x) <-> Q}) : {phi:form & representsP phi rho (proj1 H)} -> {phi:form & @representsP 0 phi rho Q}.
+Proof.
+intros [phi pR]. destruct H as [PP [eql eqr]]. cbn in pR.
+pose (∀ phi). exists f. split.
+* intros H q. destruct (pR q) as [pRl pRr]. now apply pRl, eqr, H.
+* intros H. apply eql. intros q. destruct (pR q) as [pRl pRr]. now apply pRr, H.
+Defined.
 
-MetaCoq Test Quote False.
+
+(*
+Definition representForallP (Q:Prop) := a <- tmQuote (Q);; aa <- abstractForall a;;p <- tmUnquoteTyped ({P:naryProp 1 & (forall d:D, P d) <-> Q}) aa;; ret p.
+
+MetaCoq Run (let Q:=forall x:D, x i= iO in 
+    representForallP Q).
+
+Ltac representForall k:= match goal with [ k : ?Q |- _ ] =>
+  let fr := fresh "rep" in let kkk := fresh "sml" in let pr := fresh "denv" in let k y := (pose y as fr) in
+  (run_template_program (representForallP Q) k)
+  end.
+
+Lemma stuff : true.
+pose (forall x:nat, x > 0).
+(run_template_program (representForallP (forall x : D, x i= iO)) (let k y := (pose y) in k)).
+
+
+Definition lol := iO.
+MetaCoq Quote Definition lolEnv := (fun n:nat => lol).
+Definition phiRepr (rho:nat -> D) (t:D) := {phi:term & representsF t phi rho}.
+MetaCoq Run (let trm := lol i⊕ (iσ iO) in a <- tmQuote (trm);;
+v <- findTermRepresentation FUEL a lolEnv (fun _:Ast.term => ret 0);;k<-tmUnquoteTyped (phiRepr (fun n:nat => lol) trm) v;;tmDefinition "aa" k).
+*)
+
+Definition envTermReifier := list Ast.term -> nat -> Ast.term -> (Ast.term -> TemplateMonad nat) -> (Ast.term -> TemplateMonad (prod form Ast.term)) -> TemplateMonad (prod form Ast.term).
+Definition refiyEq : envTermReifier := fun l fuel envTerm env fPR => match l with [x; y] =>  
+                                           v <- tmQuote mergeEq;;
+                                           '(tx,xr) <- findTermRepresentation fuel x envTerm env ;;
+                                           '(ty,yr) <- findTermRepresentation fuel y envTerm env ;; 
+                                           ret (tx==ty,tApp v ([envTerm;x;y;xr;yr])) | _ => tmFail "Eq constructor applied to != 2 terms" end.
+Definition reifyForm (n:nat) : envTermReifier := match n with 0 => refiyEq | _ => fun _ _ _ _ _ => tmFail ("Unknown form constructor index " ++ string_of_nat n) end.
+
 Notation baseLogicConn x l:= (tInd {| inductive_mind := (MPfile (["Logic"; "Init"; "Coq"]), x); inductive_ind := 0 |} l).
+Definition baseConnectiveReifier := list Ast.term -> nat -> Ast.term -> (Ast.term -> TemplateMonad nat) -> (Ast.term -> nat -> Ast.term -> (Ast.term -> TemplateMonad nat) -> TemplateMonad (prod form Ast.term))-> TemplateMonad (prod form Ast.term).
+Definition reifyAnd : baseConnectiveReifier := fun lst _ envTerm env fPR => match lst with [x; y] => v <- tmQuote mergeAnd;;
+                                           '(tx,xr) <- fPR x 0 envTerm env;;'(ty,yr) <- fPR y 0 envTerm env;; ret (tx∧ty,tApp v ([envTerm;x;y;xr;yr])) | _ => tmFail "And applied to != 2 terms" end.
+Definition reifyOr  : baseConnectiveReifier := fun lst _ envTerm env fPR => match lst with [x; y] => v <- tmQuote mergeOr;;
+                                           '(tx,xr) <- fPR x 0 envTerm env;;'(ty,yr) <- fPR y 0 envTerm env;; ret (tx∨ty,tApp v ([envTerm;x;y;xr;yr])) | _ => tmFail "Or applied to != 2 terms" end.
+Definition reifyExist:baseConnectiveReifier := fun lst _ envTerm env fPR => match lst with [_; P] => v <- tmQuote mergeExists;;
+                                           '(tP,rr) <- fPR P 1 envTerm env;; ret (∃ tP,tApp v ([envTerm;P;rr])) | _ => tmFail "Exist applied to wrong terms" end.
+Definition refiyCoqEq : baseConnectiveReifier := fun l fuel envTerm env fPR => match l with [tVar "D"; x; y] =>  
+                                           v <- tmQuote mergeEqProp;;
+                                           '(tx,xr) <- findTermRepresentation fuel x envTerm env ;;
+                                           '(ty,yr) <- findTermRepresentation fuel y envTerm env ;; 
+                                           ret (tx==ty,tApp v ([envTerm;x;y;xr;yr])) | _ => tmFail "Eq constructor applied to != 2 terms" end.
+Definition reifyBase (s:string) : baseConnectiveReifier := match s with "and" => reifyAnd | "or" => reifyOr | "ex" => reifyExist | "eq" => refiyCoqEq | _ => fun _ _ _ _ _ => tmFail ("Unknown connective "++s) end.
 
-Definition baseConnectiveReifier := list Ast.term -> (nat -> TemplateMonad term) -> (Ast.term -> nat -> (nat -> TemplateMonad term) -> TemplateMonad form)-> TemplateMonad form.
-Definition reifyAnd : baseConnectiveReifier := fun lst env fPR => match lst with [x; y] => 
-                                           xr <- fPR x 0 env;;yr <- fPR y 0 env;; ret (xr ∧ yr) | _ => tmFail "And applied to != 2 terms" end.
-Definition reifyOr  : baseConnectiveReifier := fun lst env fPR => match lst with [x; y] => 
-                                           xr <- fPR x 0 env;;yr <- fPR y 0 env;; ret (xr ∨ yr) | _ => tmFail "Or applied to != 2 terms" end.
-Definition reifyExist:baseConnectiveReifier := fun lst env fPR => match lst with [_; tLambda _ _ x] =>
-                                           rr <- fPR x 0 (appendAndLift (ret (var 0)) env);; ret (∃ rr) | _ => tmFail "Exist applied to wrong terms" end.
-Definition reifyBase (s:string) : baseConnectiveReifier := match s with "and" => reifyAnd | "or" => reifyOr | "ex" => reifyExist | _ => fun _ _ _ => tmFail ("Unknown connective "++s) end.
 
-MetaCoq Test Quote (False).
-MetaCoq Test Quote (and False False).
-MetaCoq Test Quote (or False False).
-MetaCoq Test Quote (False -> False).
-MetaCoq Test Quote (exists (x:D), False).
-MetaCoq Test Quote (forall (x:D), False).
+Fixpoint raiseRelIndex (minn:nat) (t:Ast.term) : Ast.term := match t with
+  tRel n => if Compare_dec.le_gt_dec minn n then tRel (S n) else tRel n
+| tVar k => tVar k
+| tEvar n ls => tEvar n (map (raiseRelIndex minn) ls)
+| tSort u => tSort u
+| tCast t ck t2 => tCast (raiseRelIndex minn t) ck (raiseRelIndex minn t2)
+| tProd n t v => tProd n (raiseRelIndex minn t) (raiseRelIndex (S minn) v)
+| tLambda n t v => tLambda n (raiseRelIndex minn t) (raiseRelIndex (S minn) v)
+| tLetIn n t v e => tLetIn n (raiseRelIndex minn t) (raiseRelIndex minn v) (raiseRelIndex (S minn) e)
+| tApp f al => tApp f (map (raiseRelIndex minn) al)
+| tConst a b => tConst a b
+| tInd i t => tInd i t
+| tConstruct a b c => tConstruct a b c
+| tCase k i r m => tCase k (raiseRelIndex minn i) (raiseRelIndex minn r) (map (fun '(a,b) => (a,raiseRelIndex minn b)) m)
+| tProj p t => tProj p (raiseRelIndex minn t)
+| tFix mft n => tFix (map (map_def (raiseRelIndex minn) (raiseRelIndex (S minn))) mft) n
+| tCoFix mft n => tCoFix (map (map_def (raiseRelIndex minn) (raiseRelIndex (S minn))) mft) n
+end.
 
-Fixpoint findPropRepresentation (fuel:nat) (t:Ast.term) (frees:nat) (env:nat->TemplateMonad term) {struct fuel}: (TemplateMonad (form)) := 
+
+Notation qProp := (tSort (Universe.from_kernel_repr (Level.lProp, false) nil)).
+
+MetaCoq Quote Definition qnaryProp1 := Eval compute in (naryProp 1).
+MetaCoq Quote Definition qexistT := @existT.
+MetaCoq Quote Definition qiff := @iff.
+MetaCoq Quote Definition qcong := @conj.
+(*MetaCoq Test Quote (@existT (naryProp 1) (fun P => (forall d:D, P d) <-> (forall d:D,False)) (fun _ => False) (conj (fun (k:(forall d:D,False))=>k) (fun (k:(forall d:D,False))=>k))).*)
+
+Definition abstractForall (t:Ast.term) : TemplateMonad (Ast.term) :=
+match t with tProd x t v =>
+    let prop := tLambda x t v in
+    let raisedV := raiseRelIndex 0 (tProd x t v) in
+    ret (tApp (qexistT) ([qnaryProp1; tLambda (nNamed "P") qnaryProp1 (tApp qiff 
+                ([tProd x t (tApp (tRel 1) ([tRel 0])); raisedV]));
+                 tLambda x t v; tApp qcong ([
+tProd (nNamed "x") (tProd x t v) raisedV;
+tProd (nNamed "x") (tProd x t v) raisedV;
+tLambda (nNamed "k") (tProd x t v) (tRel 0);
+tLambda (nNamed "k") (tProd x t v) (tRel 0)
+])]))
+| _ => tmPrint t;;tmFail "called abstractForall on something not a product" end.
+
+
+Definition pred (n:nat) := match n with 0 => 0 | S n => n end.
+Fixpoint flatten_monad {A:Type} (l:list (TemplateMonad A)) : TemplateMonad (list A) := match l with nil => ret nil | x::xr => xm <- x;; xrm <- flatten_monad xr;; ret (xm::xrm) end.
+Definition map_monad {A B:Type} (f:A -> TemplateMonad B) (l:list A) : TemplateMonad (list B) := flatten_monad (map f l).
+Definition map_def_monad {A B : Type} (tyf bodyf : A -> TemplateMonad B) (d:def A) : TemplateMonad (def B) := dtr <- tyf (dbody d);;dbr <- bodyf (dbody d);; ret {|
+dname := dname d;
+dtype := dtr;
+dbody := dbr;
+rarg := rarg d |}.
+Check (Compare_dec.le_gt_dec).
+Fixpoint lowerRelIndex (minn:nat) (tv:TemplateMonad Ast.term) (t:Ast.term) {struct t}: TemplateMonad Ast.term := match t with
+  tRel n => if Compare_dec.le_gt_dec minn n then if Compare_dec.le_gt_dec minn (S n) then tmPrint "pred";;tmPrint (tRel (pred n));;ret (tRel (pred n)) else tmPrint (minn,n);;tv else tmPrint "inside";;ret (tRel n)
+| tVar k => ret (tVar k)
+| tEvar n ls => m <- map_monad (lowerRelIndex minn tv) ls;;ret (tEvar n m)
+| tSort u => ret (tSort u)
+| tCast t ck t2 => mt <- (lowerRelIndex minn tv t);;mt2<-(lowerRelIndex minn tv t2);;ret (tCast mt ck mt2)
+| tProd n t v => mt<-(lowerRelIndex minn tv t);;mv<-(lowerRelIndex (S minn) tv v);;ret (tProd n mt mv)
+| tLambda n t v => mt<-(lowerRelIndex minn tv t);;mv<-(lowerRelIndex (S minn) tv v);;ret (tLambda n mt mv)
+| tLetIn n t v e => mt<-(lowerRelIndex minn tv t);;mv<-(lowerRelIndex minn tv v);;me<-(lowerRelIndex (S minn) tv e);;ret (tLetIn n mt mv me)
+| tApp f al => mal<-(map_monad (lowerRelIndex minn tv) al);;ret (tApp f mal)
+| tConst a b => ret (tConst a b)
+| tInd i t => ret (tInd i t)
+| tConstruct a b c => ret (tConstruct a b c)
+| tCase k i r m => mi<-(lowerRelIndex minn tv i);;mr<-(lowerRelIndex minn tv r);;mm<-(map_monad (fun '(a,b) => mb <- lowerRelIndex minn tv b;; ret (a,mb)) m);;ret (tCase k mi mr mm)
+| tProj p t => mt<-(lowerRelIndex minn tv t);;ret (tProj p mt)
+| tFix mft n => mmft<-(map_monad (map_def_monad (lowerRelIndex minn tv) (lowerRelIndex (S minn) tv)) mft);;ret (tFix mmft n)
+| tCoFix mft n => mmft<-(map_monad (map_def_monad (lowerRelIndex minn tv) (lowerRelIndex (S minn) tv)) mft);;ret (tCoFix mmft n)
+end.
+
+Definition appendZero (env:Ast.term -> TemplateMonad nat) (zv:TemplateMonad nat) : (Ast.term -> TemplateMonad nat) := 
+      fun (t:Ast.term) => match t with tRel n => (match n with 0 => zv | S n => env (tRel n) end) | _ => tmFail "stuff" end. (*k <- lowerRelIndex 0 (tmFail "Error 1337") t;; (env k) end.*)
+Definition appendAndLift (env:Ast.term -> TemplateMonad nat) (zv:TemplateMonad nat) : (Ast.term -> TemplateMonad nat) := 
+      fun t => match t with tRel n => (match n with 0 => zv | S n => k <- env (tRel n);;ret (S k) end) | _ => tmFail "stuff2" end. (*k <- lowerRelIndex 0 (tmFail "Error 1337") t;; v <- env k;;ret (S v) end.*)
+MetaCoq Quote Definition qraiseEnvTerm := (fun (d:D) (rho:nat -> D) => d .: rho).
+Definition raiseEnvTerm (d:Ast.term) (env:Ast.term) : Ast.term := tApp (qraiseEnvTerm) ([d;raiseRelIndex 0 env]).
+
+Definition mergeFreeVarIntro (rho:nat -> D) (n:nat) (P:naryProp (S n)) (H:forall d:D, {phi:form & representsP phi (d.:rho) (P d)}) (H2:forall d:D, proj1 (H iO) = proj1 (H d)) : {phi:form & representsP phi rho P}.
+Proof.
+pose (proj1 (H (iO))). exists f. intros k. destruct (H k) as [trm prf] eqn:Heq. specialize (H2 k). rewrite Heq in H2. cbn in H2. unfold f. rewrite H2. exact prf.
+Defined.
+MetaCoq Quote Definition qform := form.
+(*
+
+Definition mergeForall2 (rho:nat -> D) (Q:naryProp 0) (H:{PP : naryProp 1 & (forall x:D, PP x) <-> Q}) : {phi:form & representsP phi rho (proj1 H)} -> {phi:form & @representsP 0 phi rho Q}.
+Proof.
+intros [phi pR]. destruct H as [PP [eql eqr]]. cbn in pR.
+pose (∀ phi). exists f. split.
+* intros H q. destruct (pR q) as [pRl pRr]. now apply pRl, eqr, H.
+* intros H. apply eql. intros q. destruct (pR q) as [pRl pRr]. now apply pRr, H.
+Defined.
+*)
+
+Fixpoint findPropRepresentation (fuel:nat) (t:Ast.term) (frees:nat) (envTerm:Ast.term) (env:Ast.term -> TemplateMonad nat) {struct fuel}: (TemplateMonad (prod form Ast.term)) := tmPrint t;;
 let fail :=tmPrint (frees,t);;tmFail ("Cannot represent form") in match fuel with 0 => tmFail "Out of fuel" | S fuel => 
   match (frees,t) with
-  (0,(baseLogicConn "False" nil)) => ret (fal)
-| (0,(tApp (baseLogicConn name nil) lst)) => reifyBase name lst env (findPropRepresentation fuel)
-| (0,tProd x (tVar "D") P) =>
-      rv <- findPropRepresentation fuel P 0 (appendAndLift (ret (var 0)) env);;
-      ret ((∀ rv))
-| (0,tProd _ P Q) =>
-      rP <- findPropRepresentation fuel P 0 env;;
-      rQ <- findPropRepresentation fuel Q 0 (appendZero (tmFail "Used var of implication precondition") env);;
-      ret (rP --> rQ)
-| (0,propConstructorBase l) => match popListStart l termPropRepStart with
-        Some (formRepDet i v) => vr <- recoverVector v;;reifyForm i vr fuel env(fun t => findPropRepresentation fuel t frees env)
+  (0,(baseLogicConn "False" nil)) => v <- tmQuote mergeFalse;;ret (fal,tApp v ([envTerm]))
+| (0,(tApp (baseLogicConn name nil) lst)) => reifyBase name lst fuel envTerm env (findPropRepresentation fuel)
+| (0,(tApp propConstructorBase lst)) => match popListStart lst termPropRepStart with
+        Some (formRepDet i v) => vr <- recoverVector v;;reifyForm i vr fuel envTerm env (fun t => findPropRepresentation fuel t frees envTerm env)
       | _ => fail end
+| (0,tProd x (tVar "D") Q) =>
+      k <- abstractForall (tProd x (tVar "D") Q);;
+      '(frm,tQ) <- findPropRepresentation fuel (tLambda x (tVar "D") Q) 1 envTerm env;;
+      v <- tmQuote mergeForall2;;
+      ret (∀ frm, tApp v ([envTerm;tProd x (tVar "D") Q;k;tQ]))
+| (0,tProd _ P Q) =>
+      v <- tmQuote mergeImpl;;
+      '(tP,rP) <- findPropRepresentation fuel P 0 envTerm env;;
+      Ql <- lowerRelIndex 0 (tmFail "Used var of implication precondition") Q;;
+      '(tQ,rQ) <- findPropRepresentation fuel Ql 0 envTerm env;;
+      ret (tP --> tQ,tApp v ([envTerm;P;Ql;rP;rQ]))
 | (S n,tLambda x (tVar "D") P) => 
-      rv <- findPropRepresentation fuel P n (appendAndLift (ret (var 0)) env);;
-      ret (rv)
+      let envTermSub := raiseEnvTerm (tRel 0) envTerm in
+      let envSub := appendAndLift env (ret 0) in
+      '(frm,k) <- findPropRepresentation fuel P n envTermSub envSub;;
+      v <- tmQuote mergeFreeVarIntro;;
+      num <- tmQuote n;;
+      vfrmq <- tmQuote frm;;
+      ret (frm,tApp v ([envTerm;num;tLambda x (tVar "D") P;tLambda x (tVar "D") k;tLambda x (tVar "D") (tApp qeq_refl ([qform;vfrmq]))]))
 | _ => fail end end.
 
-(*MetaCoq  Run (a <- tmQuote (iσ (iσ iO));; k <- findTermRepresentation a;; tmDefinition "res" k).*)
-(*MetaCoq  Run (a <- tmQuote (forall (x:D), x i= x);; k <- findPropRepresentation a failEnv;; tmPrint k).*)
+Check print_term.
+MetaCoq Quote Recursively Definition k := mergeFreeVarIntro.
+Check (fst k).
+Definition genv := empty_ext (fst k).
 
+Ltac representEnv env := match goal with [ |- representableP ?n ?G ] =>
+  let rep := fresh "rep" in let prf := fresh "prf" in let hyp := fresh "H" in let k y := (idtac y;destruct y as [rep prf]) in
+  (run_template_program (g <- (tmQuote G);;qe <- tmQuote env;;'(aaa,rp)<-findPropRepresentation FUEL g n qe (fun v => tmFail "unbound");;tmPrint (aaa,rp);;(*print_term genv nil false rp*)tmUnquoteTyped ({phi:form & @representsP n phi env G}) rp) k)
+  ;exists rep;exists env;exact prf
+end.
+Ltac represent := representEnv (fun k:nat => iO).
 
-Ltac represent:= match goal with [ |- representableP ?n ?G ] =>
-  let fr := fresh "rep" in let kkk := fresh "sml" in let pr := fresh "denv" in let k y := (pose y as fr) in
-  (run_template_program (g <- (tmQuote G);;findPropRepresentation FUEL g n failEnv) k)
-  ;exists fr; pose (fun (_:nat) => iO) as pr; exists pr; split; easy
-  end.
+Goal (representableP 0 (iO i= iO)).
+represent.
+Qed.
+
+Goal (representableP 0 (forall d:D, d i= iO)).
+represent.
+Qed.
+
+Goal (representableP 1 (fun a => False -> a i= a)).
+represent.
+Qed.
 
 Goal (representableP 2 (fun (d e :D) => forall g, exists j, g i= d i⊕ j /\ False -> False \/ (e i⊗ e i= iσ j /\ False))).
 represent.
+
+
+Goal (forall n:nat, representableF (iμ n)).
+intros n. induction n as [|n [phi [rho IH]]].
+* cbn. exists zero. pose (fun (n:nat) => iO). exists d. split.
+* cbn. unfold representableF. pose (σ phi). exists t. exists rho. unfold representsF. unfold representsF in IH. unfold t. cbn. now rewrite IH.
 Qed.
 
   Lemma sat_single (rho : nat -> D) (Phi : form) (t : term) :
@@ -323,25 +542,17 @@ Qed.
     apply zero_or_succ.
   Qed.
 
-  Goal forall d, iO = d \/ exists x, d = iσ x. 
+  Goal forall d, iO i= d \/ exists x, d i= iσ x. 
   Proof.
-    apply PAinduction.
-    pose (phi := zero == $0 ∨ ∃ $1 == σ $0).
-    - exists phi, (fun _ => iO). split.
-      + intros [<- | [x ->]].
-        * left. cbn. now rewrite equality.
-        * right. exists x. cbn. now rewrite equality.
-      + intros [H | [x H]].
-        * left. cbn in H. now rewrite equality in H.
-        * right. exists x. cbn in H. now rewrite equality in H.
-    - now left.
-    - intros d [<- |]; right. now exists iO. now exists d.
+    apply PAinduction. represent.
+    - left. now rewrite equality.
+    - intros d [HL |]. rewrite equality in HL. cbn in HL. rewrite <- HL. right. pose iO as miO. exists miO. rewrite equality. easy. right. exists d. rewrite equality. easy.
   Qed.
 
   Lemma add_rec_right :
-    forall d n, n i⊕ (iσ d) = iσ (n i⊕ d).
+    forall d n, n i⊕ (iσ d) i= iσ (n i⊕ d).
   Proof.
-    intros n. apply PAinduction.
+    apply PAinduction.
     - represent. pose (phi := ∀ $1 ⊕ σ $2 == σ ($1 ⊕ $2) ).
       exists phi. exists (fun _ => n). intros d. cbn. split.
       + intros H d0. rewrite equality. cbn. easy.
